
% \begin{verbatim}
% Forall q#3 . q#3 = 10 =>
%     Forall r#1 . r#1 = 55 =>
%         (q#3 >= 0 /\ r#1 >= 0) /\ Forall res#3 . res#3 = 0 =>
%             Forall ghosta . ghosta = q#3 =>
%                 res#3 = (ghosta - q#3) * r#1 /\ Forall q#1 . Forall res#1 .
%                     (q#1 >= 0 /\ res#1 = (ghosta - q#1) * r#1) =>
%                         Forall res#2 . res#2 = res#1 + r#1 =>
%                             Forall q#2 . q#2 = q#1 - 1 =>
%                               res#2 = (ghosta - q#2) * r#1
%                         /\ (q#1 <= 0 /\ res#1 = (ghosta - q#1) * r#1) =>
%                               res#1 = ghosta * r#1
% \end{verbatim}

% \begin{align*}
%          &\forall q\#3 . q\#3 = 10 \Rightarrow \\
%          &\quad \forall r\#1 . r\#1 = 55 \Rightarrow \\
%          &\quad \quad (q\#3 \geq 0 \land r\#1 \geq 0)
%          							\land \forall res\#3 . res\#3 = 0 \Rightarrow \\
%          &\quad \quad \quad \quad \forall ghosta . ghosta = q\#3 \Rightarrow \\
%          &\quad \quad \quad \quad \quad res\#3 = (ghosta - q\#3) \cdot r\#1 \\
%          &\quad \quad \quad \quad \quad \land
%            \forall q\#1 . \forall res\#1 .
%               (q\#1 \geq 0 \land res\#1 = (ghosta - q\#1) \cdot r\#1) \Rightarrow \\
%          &\quad \quad \quad \quad \quad \quad
%            \forall res\#2 . res\#2 = res\#1 + r\#1 \Righarrow \\
%          &\quad \quad \quad \quad \quad \quad \quad
%            \forall q\#2 . q\#2 = q\#1 - 1 \Rightarrow \\
%          &\quad \quad \quad \quad \quad \quad \quad \quad
%            res\#2 = (ghosta - q\#2) \cdot r\#1 \\
%          &\quad \quad \quad \quad \quad \quad \land
%            (q\#1 \leq 0 \land res\#1 = (ghosta - q\#1) \cdot r\#1) \Rightarrow \\
%          &\quad \quad \quad \quad \quad \quad \quad
%            res\#1 = ghosta \cdot r\#1
% \end{align*}


% \begin{lstlisting}
% Forall q#3 . q#3 = 10 =>
%     Forall r#1 . r#1 = 55 =>
%         (q#3 >= 0 /\ r#1 >= 0) /\ Forall res#3 . res#3 = 0 =>
%             Forall ghosta . ghosta = q#3 =>
%                 res#3 = (ghosta - q#3) * r#1
%                 /\
%                 Forall q#1 . Forall res#1 .
%                     (q#1 >= 0 /\ res#1 = (ghosta - q#1) * r#1) =>
%                         Forall res#2 . res#2 = res#1 + r#1 =>
%                             Forall q#2 . q#2 = q#1 - 1 =>
%                                 res#2 = (ghosta - q#2) * r#1
%                         /\
%                         (q#1 <= 0 /\ res#1 = (ghosta - q#1) * r#1) =>
%                             res#1 = ghosta * r#1
% \end{lstlisting}
\begin{lstlisting}[mathescape=true, escapechar=@]
  $\forall q, r. \; (q \geq 0) \Rightarrow$
  $ \quad \forall res_{3}. \; res_{3} = 0 \Rightarrow$
  $\quad \quad \forall ðŸ‘»a. \; ðŸ‘»a = q \Rightarrow$
  $\quad \quad \quad (res_{3} = (ðŸ‘»a - q) * r \land q \geq 0)$
  $\quad \quad \quad \; \land \forall q_{2}, res_{2}, \xi_{1}.$
  $\quad \quad \quad \quad (q_{2} > 0 \land res_{2} = (ðŸ‘»a - q_{2}) * r \land q_{2} \geq 0 \land \xi_{1} = q_{2}) \Rightarrow$
  $\quad \quad \quad \quad \quad \forall res_{1}. \; res_{1} = res_{2} + r \Rightarrow$
  $\quad \quad \quad \quad \quad \quad \forall q_{1}. \, q_{1} = q_{2} - 1 \Rightarrow$
  $\quad \quad \quad \quad \quad \quad \quad (res_{1} = (ðŸ‘»a - q_{1}) * r \land q_{1} \geq 0 \land 0 \leq \xi_{1} \land q_{1} < \xi_{1})$
  $\quad \quad \quad \land ((q_{2} \leq 0 \land res_{2} = (ðŸ‘»a - q_{2}) * r \land q_{2} \geq 0) => res_{2} = ðŸ‘»a * r)$
  \end{lstlisting}
% \begin{lstlisting}[mathescape=true]
% $\forall \, q_3, \, (q_3 = 10) \Rightarrow$
% $\quad \forall r_1 , r_1 = 55 \Rightarrow$
% $\quad \quad (q_3 \geq 0 \land r_1 \geq 0)
% 						\land \forall \, res_3 , \, res_3 = 0 \Rightarrow$
% $\quad \quad \quad \quad \forall \, ghosta, \, (ghosta = q_3) \Rightarrow$
% $\quad \quad \quad \quad \quad res_3 = (ghosta - q_3) \cdot r_1$
% $\quad \quad \quad \quad \quad \land
%          \forall q_1 , \forall res_1 , \,
%              (q_1 \geq 0 \land res_1 = (ghosta - q_1) \cdot r_1) \Rightarrow$
% $ \quad \quad \quad \quad \quad \quad
%         \forall res_2 , \, res_2 = (res_1 + r_1) \Rightarrow $
% $ \quad \quad \quad \quad \quad \quad \quad
%           \forall q_2 , q_2 = (q_1 - 1) \Rightarrow$
% $\quad \quad \quad \quad \quad \quad \quad \quad
%           res_2 = (ghosta - q_2) \cdot r_1$
% $\quad \quad \quad \quad \quad \quad \land
%           (q_1 \leq 0 \land res_1 = (ghosta - q_1) \cdot r_1) \Rightarrow$
% $\quad \quad \quad \quad \quad \quad \quad res_1 = ghosta \cdot r_1$
% \end{lstlisting}
